uniformize UntypedIndSemantics

coq/UntypedIndSemantics.v
@@ -1,120 +1,112 @@
 (*! Language | Semantics of typed Kôika programs !*)
-Require Export Koika.Common Koika.Environments Koika.ULogs Koika.Syntax
-        Koika.Syntax.
-Require Import Desugaring.
-Require Import SyntaxMacros.
-Require Import UntypedSemantics.
-Require Import BitsToLists.
 Require Import Coq.Program.Equality.
+Require Export Koika.Common Koika.Environments Koika.Syntax Koika.ULogs.
+Require Import BitsToLists Desugaring SyntaxMacros UntypedSemantics.
 
 Section Interp.
   Context {pos_t var_t fn_name_t: Type}.
   Context `{var_t_eq_dec: EqDec var_t}.
 
   Inductive interp_list
-            {reg_t ext_fn_t: Type}
-            {REnv: Env reg_t}
-            (r: REnv.(env_t) (fun _ => val))
-            (sigma: forall f: ext_fn_t, val -> val)
-            (i: forall     (Gamma: list (var_t * val))
-                           (sched_log: Log REnv)
-                           (action_log: Log REnv)
-                           (a: Syntax.uaction pos_t var_t fn_name_t reg_t ext_fn_t)
-                           (action_log': Log REnv)
-                           (res: val)
-                           (Gamma': list (var_t * val)), Prop):
-    forall
-      (Gamma: list (var_t * val))
-      (sched_log: Log REnv)
-      (action_log: Log REnv)
+    {reg_t ext_fn_t: Type} {REnv: Env reg_t} (r: REnv.(env_t) (fun _ => val))
+    (sigma: forall f: ext_fn_t, val -> val)
+    (i: forall
+      (Gamma: list (var_t * val)) (sched_log: Log REnv) (action_log: Log REnv)
+      (a: Syntax.uaction pos_t var_t fn_name_t reg_t ext_fn_t)
+      (action_log': Log REnv) (res: val) (Gamma': list (var_t * val)), Prop
+    )
+  : forall
+      (Gamma: list (var_t * val)) (sched_log: Log REnv) (action_log: Log REnv)
       (a: list (Syntax.uaction pos_t var_t fn_name_t reg_t ext_fn_t))
-      (action_log': Log REnv)
-      (res: list val)
-      (Gamma': list (var_t * val)), Prop :=
+      (action_log': Log REnv) (res: list val) (Gamma': list (var_t * val)), Prop
+  :=
   | interp_list_nil:
-      forall (Gamma: list (var_t * val))
-             (sched_log: Log REnv)
-             (action_log: Log REnv),
-        interp_list r sigma i Gamma sched_log action_log [] action_log [] Gamma
+    forall
+      (Gamma: list (var_t * val)) (sched_log: Log REnv) (action_log: Log REnv),
+    interp_list r sigma i Gamma sched_log action_log [] action_log [] Gamma
   | interp_list_cons:
-      forall (Gamma: list (var_t * val))
-             (sched_log: Log REnv)
-             (action_log: Log REnv)
-             Gamma' action_log' Gamma'' action_log'' a ar v vr,
-        i Gamma sched_log action_log a action_log' v Gamma' ->
-        interp_list r sigma i Gamma' sched_log action_log' ar action_log'' vr Gamma'' ->
-        interp_list r sigma i Gamma sched_log action_log (a::ar) action_log'' (vr++[v]) Gamma''
-  .
+    forall
+      (Gamma: list (var_t * val)) (sched_log: Log REnv) (action_log: Log REnv)
+      Gamma' action_log' Gamma'' action_log'' a ar v vr,
+    i Gamma sched_log action_log a action_log' v Gamma' ->
+    interp_list
+      r sigma i Gamma' sched_log action_log' ar action_log'' vr Gamma''
+    -> interp_list
+      r sigma i Gamma sched_log action_log (a::ar) action_log'' (vr++[v])
+      Gamma''.
 
   Lemma fold_left_rec:
-    forall {reg_t ext_fn_t: Type}
-           {REnv: Env reg_t}
-           (f: forall     (Gamma: list (var_t * val))
-                     (sched_log: Log REnv)
-                     (action_log: Log REnv)
-                     (a: Syntax.uaction pos_t var_t fn_name_t reg_t ext_fn_t),
-          option (Log REnv * val * list (var_t * val)))
-           (sched_log: Log REnv) l X action_log Gamma,
-      fold_left (fun acc a =>
-                   let/opt3 action_log, l, Gamma := acc in
-                   let/opt3 action_log, v, Gamma :=
-                      f Gamma sched_log action_log a in
-                   Some (action_log, v::l, Gamma))
-                l
-                (Some (action_log, X, Gamma)) =
-      match     fold_left (fun acc a =>
-                             let/opt3 action_log, l, Gamma := acc in
-                             let/opt3 action_log, v, Gamma :=
-                                f Gamma sched_log action_log a in
-                             Some (action_log, v::l, Gamma))
-                          l
-                          (Some (action_log, [], Gamma)) with
-        None => None
-      | Some (al, l, Gamma) => Some (al, l ++ X, Gamma)
-      end.
+    forall
+      {reg_t ext_fn_t: Type} {REnv: Env reg_t}
+      (f: forall (Gamma: list (var_t * val)) (sched_log: Log REnv)
+      (action_log: Log REnv)
+      (a: Syntax.uaction pos_t var_t fn_name_t reg_t ext_fn_t),
+    option
+      (Log REnv * val * list (var_t * val)))
+      (sched_log: Log REnv) l X action_log Gamma,
+    fold_left
+      (fun acc a =>
+        let/opt3 action_log, l, Gamma := acc in
+        let/opt3 action_log, v, Gamma := f Gamma sched_log action_log a in
+        Some (action_log, v::l, Gamma)
+      )
+      l (Some (action_log, X, Gamma))
+    = match fold_left
+      (fun acc a =>
+        let/opt3 action_log, l, Gamma := acc in
+        let/opt3 action_log, v, Gamma := f Gamma sched_log action_log a in
+        Some (action_log, v::l, Gamma)
+      )
+      l (Some (action_log, [], Gamma))
+    with
+    | None => None
+    | Some (al, l, Gamma) => Some (al, l ++ X, Gamma)
+    end.
   Proof.
     induction l; simpl; intros; eauto.
-    destruct (f Gamma sched_log action_log a) eqn:?; simpl; auto. destruct p. destruct p.
+    destruct (f Gamma sched_log action_log a) eqn:?; simpl; auto.
+    destruct p. destruct p.
     rewrite (IHl (v::X)).
     rewrite (IHl [v]).
     destr. repeat destr. rewrite <- app_assoc. simpl. auto.
     rewrite fold_left_none. auto. simpl; auto.
   Qed.
-  
+
   Lemma interp_list_ok:
     forall
-      {reg_t ext_fn_t: Type}
-      {REnv: Env reg_t}
-      (r: REnv.(env_t) (fun _ => val))
+      {reg_t ext_fn_t: Type} {REnv: Env reg_t} (r: REnv.(env_t) (fun _ => val))
       (sigma: forall f: ext_fn_t, val -> val)
-      (i: forall     (Gamma: list (var_t * val))
-                     (sched_log: Log REnv)
-                     (action_log: Log REnv)
-                     (a: Syntax.uaction pos_t var_t fn_name_t reg_t ext_fn_t)
-                     (action_log': Log REnv)
-                     (res: val)
-                     (Gamma': list (var_t * val)), Prop)
-      (f: forall     (Gamma: list (var_t * val))
-                     (sched_log: Log REnv)
-                     (action_log: Log REnv)
-                     (a: Syntax.uaction pos_t var_t fn_name_t reg_t ext_fn_t),
-          option (Log REnv * val * list (var_t * val)))
+      (i: forall
+          (Gamma: list (var_t * val)) (sched_log: Log REnv)
+          (action_log: Log REnv)
+          (a: Syntax.uaction pos_t var_t fn_name_t reg_t ext_fn_t)
+          (action_log': Log REnv) (res: val) (Gamma': list (var_t * val)),
+        Prop
+      )
+      (f: forall
+          (Gamma: list (var_t * val)) (sched_log: Log REnv)
+          (action_log: Log REnv)
+          (a: Syntax.uaction pos_t var_t fn_name_t reg_t ext_fn_t),
+        option (Log REnv * val * list (var_t * val))
+      )
       l
       (iok:
-         forall Gamma sched_log action_log Gamma' action_log' a v,
-           In a l ->
-           f Gamma sched_log action_log a = Some (action_log', v, Gamma') <->
-           i Gamma sched_log action_log a action_log' v Gamma'
+        forall Gamma sched_log action_log Gamma' action_log' a v,
+        In a l
+        -> f Gamma sched_log action_log a = Some (action_log', v, Gamma')
+        <-> i Gamma sched_log action_log a action_log' v Gamma'
       ),
     forall Gamma action_log sched_log action_log' Gamma' lv,
-      fold_left (fun acc a =>
-                        let/opt3 action_log, l, Gamma := acc in
-                        let/opt3 action_log, v, Gamma :=
-                           f Gamma sched_log action_log a in
-                        Some (action_log, v::l, Gamma))
-                     l
-                     (Some (action_log, [], Gamma)) = Some (action_log', lv, Gamma') <->
-      interp_list r sigma i Gamma sched_log action_log l action_log' lv Gamma'.
+      fold_left
+        (fun acc a =>
+          let/opt3 action_log, l, Gamma := acc in
+          let/opt3 action_log, v, Gamma := f Gamma sched_log action_log a in
+          Some (action_log, v::l, Gamma)
+        )
+        l (Some (action_log, [], Gamma))
+      = Some (action_log', lv, Gamma')
+      <-> interp_list
+        r sigma i Gamma sched_log action_log l action_log' lv Gamma'.
   Proof.
     induction l; simpl; intros; eauto.
     - split; intro A; inv A. constructor. auto.
@@ -142,74 +134,69 @@ Section Interp.
         rewrite <- iok in H4. congruence. auto.
   Qed.
 
-
   Inductive interp_list_ctx
-            {reg_t ext_fn_t: Type}
-            {REnv: Env reg_t}
-            (r: REnv.(env_t) (fun _ => val))
-            (sigma: forall f: ext_fn_t, val -> val)
-            (i: forall     (Gamma: list (var_t * val))
-                           (sched_log: Log REnv)
-                           (action_log: Log REnv)
-                           (a: Syntax.uaction pos_t var_t fn_name_t reg_t ext_fn_t)
-                           (action_log': Log REnv)
-                           (res: val)
-                           (Gamma': list (var_t * val)), Prop):
-    forall
-      (Gamma: list (var_t * val))
-      (sched_log: Log REnv)
-      (action_log: Log REnv)
+    {reg_t ext_fn_t: Type} {REnv: Env reg_t} (r: REnv.(env_t) (fun _ => val))
+    (sigma: forall f: ext_fn_t, val -> val)
+    (i: forall
+      (Gamma: list (var_t * val)) (sched_log: Log REnv) (action_log: Log REnv)
+      (a: Syntax.uaction pos_t var_t fn_name_t reg_t ext_fn_t)
+      (action_log': Log REnv) (res: val) (Gamma': list (var_t * val)), Prop
+    )
+  : forall
+      (Gamma: list (var_t * val)) (sched_log: Log REnv) (action_log: Log REnv)
       (a: list (var_t * Syntax.uaction pos_t var_t fn_name_t reg_t ext_fn_t))
-      (action_log': Log REnv)
-      (Gamma': list (var_t * val)), Prop :=
+      (action_log': Log REnv) (Gamma': list (var_t * val)),
+    Prop
+  :=
   | interp_list_ctx_nil:
-      forall (Gamma: list (var_t * val))
-             (sched_log: Log REnv)
-             (action_log: Log REnv),
-        interp_list_ctx r sigma i Gamma sched_log action_log [] action_log Gamma
-  | interp_list_ctx_cons:
-      forall (Gamma: list (var_t * val))
-             (sched_log: Log REnv)
-             (action_log: Log REnv)
-             Gamma' action_log' Gamma'' action_log'' var a ar v,
-        i Gamma sched_log action_log a action_log' v Gamma' ->
-        interp_list_ctx r sigma i ((var,v)::Gamma') sched_log action_log' ar action_log'' Gamma'' ->
-        interp_list_ctx r sigma i Gamma sched_log action_log ((var,a)::ar) action_log'' Gamma''
-  .
-
-   Lemma interp_list_ctx_ok:
     forall
-      {reg_t ext_fn_t: Type}
-      {REnv: Env reg_t}
-      (r: REnv.(env_t) (fun _ => val))
+      (Gamma: list (var_t * val)) (sched_log: Log REnv) (action_log: Log REnv),
+    interp_list_ctx r sigma i Gamma sched_log action_log [] action_log Gamma
+  | interp_list_ctx_cons:
+    forall
+      (Gamma: list (var_t * val)) (sched_log: Log REnv) (action_log: Log REnv)
+      Gamma' action_log' Gamma'' action_log'' var a ar v,
+    i Gamma sched_log action_log a action_log' v Gamma'
+    -> interp_list_ctx
+      r sigma i ((var,v)::Gamma') sched_log action_log' ar action_log'' Gamma''
+    -> interp_list_ctx
+      r sigma i Gamma sched_log action_log ((var,a)::ar) action_log'' Gamma''.
+
+  Lemma interp_list_ctx_ok:
+    forall
+      {reg_t ext_fn_t: Type} {REnv: Env reg_t} (r: REnv.(env_t) (fun _ => val))
       (sigma: forall f: ext_fn_t, val -> val)
-      (i: forall     (Gamma: list (var_t * val))
-                     (sched_log: Log REnv)
-                     (action_log: Log REnv)
-                     (a: Syntax.uaction pos_t var_t fn_name_t reg_t ext_fn_t)
-                     (action_log': Log REnv)
-                     (res: val)
-                     (Gamma': list (var_t * val)), Prop)
-      (f: forall     (Gamma: list (var_t * val))
-                     (sched_log: Log REnv)
-                     (action_log: Log REnv)
-                     (a: Syntax.uaction pos_t var_t fn_name_t reg_t ext_fn_t),
-          option (Log REnv * val * list (var_t * val)))
+      (i: forall
+          (Gamma: list (var_t * val)) (sched_log: Log REnv)
+          (action_log: Log REnv)
+          (a: Syntax.uaction pos_t var_t fn_name_t reg_t ext_fn_t)
+          (action_log': Log REnv) (res: val) (Gamma': list (var_t * val)),
+        Prop
+      )
+      (f: forall
+          (Gamma: list (var_t * val)) (sched_log: Log REnv)
+          (action_log: Log REnv)
+          (a: Syntax.uaction pos_t var_t fn_name_t reg_t ext_fn_t),
+        option (Log REnv * val * list (var_t * val))
+      )
       l
       (iok:
-         forall Gamma sched_log action_log Gamma' action_log' a v,
-           In a (map snd l) ->
-           f Gamma sched_log action_log a = Some (action_log', v, Gamma') <->
-           i Gamma sched_log action_log a action_log' v Gamma'
+        forall Gamma sched_log action_log Gamma' action_log' a v,
+        In a (map snd l)
+        -> f Gamma sched_log action_log a = Some (action_log', v, Gamma')
+        <-> i Gamma sched_log action_log a action_log' v Gamma'
       ),
     forall Gamma action_log sched_log action_log' Gamma',
-      List.fold_left (fun acc '(var, a) =>
-                             let/opt2 action_log, Gamma' := acc in
-                             let/opt3 action_log, v, Gamma' :=
-                                f Gamma' sched_log action_log a in
-                             (Some (action_log, (var,v)::Gamma'))
-                          ) l (Some (action_log, Gamma)) = Some (action_log', Gamma') <->
-      interp_list_ctx r sigma i Gamma sched_log action_log l action_log' Gamma'.
+    List.fold_left
+      (fun acc '(var, a) =>
+        let/opt2 action_log, Gamma' := acc in
+        let/opt3 action_log, v, Gamma' := f Gamma' sched_log action_log a in
+        (Some (action_log, (var,v)::Gamma'))
+      )
+      l (Some (action_log, Gamma))
+    = Some (action_log', Gamma')
+    <-> interp_list_ctx
+      r sigma i Gamma sched_log action_log l action_log' Gamma'.
   Proof.
     induction l; simpl; intros; eauto.
     - split; intros A; inv A. constructor. auto.
@@ -233,43 +220,48 @@ Section Interp.
   Qed.
 
   Lemma structinit_ind_ok:
-      forall {reg_t ext_fn_t: Type}
-           {REnv: Env reg_t}
-           (r: REnv.(env_t) (fun _ => val))
-           (sigma: forall f: ext_fn_t, val -> val)
-           (i: forall     (Gamma: list (var_t * val))
-                     (sched_log: Log REnv)
-                     (action_log: Log REnv)
-                     (a: Syntax.uaction pos_t var_t fn_name_t reg_t ext_fn_t)
-                     (action_log': Log REnv)
-                     (res: val)
-                     (Gamma': list (var_t * val)), Prop)
-      (f: forall     (Gamma: list (var_t * val))
-                     (sched_log: Log REnv)
-                     (action_log: Log REnv)
-                     (a: Syntax.uaction pos_t var_t fn_name_t reg_t ext_fn_t),
-          option (Log REnv * val * list (var_t * val)))
-      fields (iok:
-                forall Gamma sched_log action_log Gamma' action_log' a v,
-                  In a (map snd fields) ->
-           f Gamma sched_log action_log a = Some (action_log', v, Gamma') <->
-           i Gamma sched_log action_log a action_log' v Gamma'
-      ) sched_log
-       Gamma Gamma' action_log action_log' vs v sig,
-        (exists vfields,
-            interp_list r sigma i
-                     Gamma sched_log action_log (map snd fields) action_log' vfields Gamma' /\
-        List.fold_left (fun vs '(name, v) =>
-                          let/opt vs := vs in
-                          subst_field_name (struct_fields sig) name v vs
-                       ) (combine (map fst fields) (rev vfields)) (Some vs) = Some v) <->
-        List.fold_left (fun acc '(name, a) =>
-                    let/opt3 action_log, vs, Gamma := acc in
-                    let/opt3 action_log, v, Gamma :=
-                       f Gamma sched_log action_log a in
-                    let/opt vs := subst_field_name (struct_fields sig) name v vs in
-                    (Some (action_log, vs, Gamma))
-                       ) fields (Some (action_log, vs, Gamma)) = Some (action_log', v, Gamma').
+    forall
+      {reg_t ext_fn_t: Type} {REnv: Env reg_t} (r: REnv.(env_t) (fun _ => val))
+      (sigma: forall f: ext_fn_t, val -> val)
+      (i: forall
+          (Gamma: list (var_t * val)) (sched_log: Log REnv)
+          (action_log: Log REnv)
+          (a: Syntax.uaction pos_t var_t fn_name_t reg_t ext_fn_t)
+          (action_log': Log REnv) (res: val) (Gamma': list (var_t * val)),
+        Prop
+      )
+      (f: forall
+          (Gamma: list (var_t * val)) (sched_log: Log REnv)
+          (action_log: Log REnv)
+          (a: Syntax.uaction pos_t var_t fn_name_t reg_t ext_fn_t),
+        option (Log REnv * val * list (var_t * val))
+      )
+      fields
+      (iok: forall Gamma sched_log action_log Gamma' action_log' a v,
+         In a (map snd fields)
+         -> f Gamma sched_log action_log a = Some (action_log', v, Gamma')
+         <-> i Gamma sched_log action_log a action_log' v Gamma'
+      )
+      sched_log Gamma Gamma' action_log action_log' vs v sig,
+    (exists vfields,
+      interp_list
+        r sigma i Gamma sched_log action_log (map snd fields) action_log'
+        vfields Gamma'
+      /\ List.fold_left
+        (fun vs '(name, v) =>
+          let/opt vs := vs in subst_field_name (struct_fields sig) name v vs
+        )
+        (combine (map fst fields) (rev vfields))
+        (Some vs) = Some v
+    )
+    <-> List.fold_left
+      (fun acc '(name, a) =>
+        let/opt3 action_log, vs, Gamma := acc in
+        let/opt3 action_log, v, Gamma := f Gamma sched_log action_log a in
+        let/opt vs := subst_field_name (struct_fields sig) name v vs in
+        (Some (action_log, vs, Gamma))
+      )
+      fields (Some (action_log, vs, Gamma)) = Some (action_log', v, Gamma').
   Proof.
     induction fields; simpl; intros; eauto.
     - split; intros A. destruct A; intuition subst. inv H1. inv H0. auto.
@@ -277,7 +269,8 @@ Section Interp.
     - destr.
       destruct (f Gamma sched_log action_log u) eqn:?; simpl in *; auto.
       + destruct p, p.
-        destruct (subst_field_name (struct_fields sig) s v0 vs) eqn:?; simpl in *; auto.
+        destruct (subst_field_name (struct_fields sig) s v0 vs) eqn:?;
+        simpl in *; auto.
         * rewrite <- IHfields.
           split; intros (vfields & A & B).
           inv A.
@@ -301,57 +294,65 @@ Section Interp.
         destruct A; intuition. inv H0.
         apply iok in H6. rewrite H6 in Heqo; inv Heqo. auto.
   Qed.
-    Notation "'let/opt4' v1 ',' v2 ',' v3 ',' v4 ':=' expr 'in' body" :=
-      (opt_bind expr (fun '(v1, v2, v3, v4) => body)) (at level 200).
+
+  Notation "'let/opt4' v1 ',' v2 ',' v3 ',' v4 ':=' expr 'in' body" :=
+    (opt_bind expr (fun '(v1, v2, v3, v4) => body)) (at level 200).
 
   Lemma arrayinit_ind_ok:
-      forall {reg_t ext_fn_t: Type}
-           {REnv: Env reg_t}
-           (r: REnv.(env_t) (fun _ => val))
-           (sigma: forall f: ext_fn_t, val -> val)
-           (i: forall     (Gamma: list (var_t * val))
-                     (sched_log: Log REnv)
-                     (action_log: Log REnv)
-                     (a: Syntax.uaction pos_t var_t fn_name_t reg_t ext_fn_t)
-                     (action_log': Log REnv)
-                     (res: val)
-                     (Gamma': list (var_t * val)), Prop)
-      (f: forall     (Gamma: list (var_t * val))
-                     (sched_log: Log REnv)
-                     (action_log: Log REnv)
-                     (a: Syntax.uaction pos_t var_t fn_name_t reg_t ext_fn_t),
-          option (Log REnv * val * list (var_t * val)))
-      elts (iok:
-                forall Gamma sched_log action_log Gamma' action_log' a v,
-                  In a elts ->
-           f Gamma sched_log action_log a = Some (action_log', v, Gamma') <->
-           i Gamma sched_log action_log a action_log' v Gamma'
-      ) sched_log
-       Gamma Gamma' action_log action_log' vs v x pos,
-        (exists velts,
-            interp_list r sigma i
-                        Gamma sched_log action_log elts action_log' velts Gamma' /\
-            List.fold_left (fun acc v =>
-                        let/opt2 pos, vs := acc in
-                             let/opt2 l1, l2 := take_drop pos vs in
-                             match l2 with
-                               [] => None
-                             | a::l2 => Some (S pos, l1 ++ v :: l2)
-                             end
-                           ) (rev velts) (Some (pos, vs)) = Some (x, v)) <->
-                   List.fold_left (fun acc a =>
-                             let/opt4 pos, action_log, vs, Gamma := acc in
-                             let/opt3 action_log, v, Gamma :=
-                                f Gamma sched_log action_log a in
-                             let/opt2 l1, l2 := take_drop pos vs in
-                             match l2 with
-                               [] => None
-                             | a::l2 => Some (S pos, action_log, l1 ++ v :: l2, Gamma)
-                             end
-                          ) elts (Some (pos, action_log, vs, Gamma)) = Some (x, action_log', v, Gamma').
+    forall
+      {reg_t ext_fn_t: Type} {REnv: Env reg_t} (r: REnv.(env_t) (fun _ => val))
+      (sigma: forall f: ext_fn_t, val -> val)
+      (i: forall
+          (Gamma: list (var_t * val)) (sched_log: Log REnv)
+          (action_log: Log REnv)
+          (a: Syntax.uaction pos_t var_t fn_name_t reg_t ext_fn_t)
+          (action_log': Log REnv) (res: val) (Gamma': list (var_t * val)),
+        Prop
+      )
+      (f: forall
+          (Gamma: list (var_t * val)) (sched_log: Log REnv)
+          (action_log: Log REnv)
+          (a: Syntax.uaction pos_t var_t fn_name_t reg_t ext_fn_t),
+        option (Log REnv * val * list (var_t * val))
+      )
+      elts
+      (iok:
+        forall Gamma sched_log action_log Gamma' action_log' a v,
+        In a elts
+        -> f Gamma sched_log action_log a = Some (action_log', v, Gamma')
+        <-> i Gamma sched_log action_log a action_log' v Gamma'
+      )
+      sched_log Gamma Gamma' action_log action_log' vs v x pos,
+    (exists velts,
+      interp_list
+        r sigma i Gamma sched_log action_log elts action_log' velts Gamma'
+        /\ List.fold_left
+          (fun acc v =>
+            let/opt2 pos, vs := acc in
+            let/opt2 l1, l2 := take_drop pos vs in
+            match l2 with
+            | []    => None
+            | a::l2 => Some (S pos, l1 ++ v :: l2)
+            end
+          )
+          (rev velts) (Some (pos, vs))
+        = Some (x, v)
+    ) <-> List.fold_left
+      (fun acc a =>
+        let/opt4 pos, action_log, vs, Gamma := acc in
+        let/opt3 action_log, v, Gamma := f Gamma sched_log action_log a in
+        let/opt2 l1, l2 := take_drop pos vs in
+        match l2 with
+        | []    => None
+        | a::l2 => Some (S pos, action_log, l1 ++ v :: l2, Gamma)
+        end
+      )
+      elts (Some (pos, action_log, vs, Gamma))
+    = Some (x, action_log', v, Gamma').
   Proof.
     induction elts; simpl; intros; eauto.
-    - split; intros A. destruct A; intuition subst. inv H0. simpl in H1. inv H1. auto.
+    - split; intros A. destruct A; intuition subst. inv H0.
+      simpl in H1. inv H1. auto.
       inv A. eexists; split. constructor. auto.
     - destruct (f Gamma sched_log action_log a) eqn:?; simpl in *; auto.
       + destruct p, p.
@@ -380,7 +381,8 @@ Section Interp.
           destruct A; intuition. inv H0.
           apply iok in H6. rewrite H6 in Heqo; inv Heqo.
           rewrite rev_app_distr in H1. simpl in H1. rewrite Heqo0 in H1.
-          simpl in H1. rewrite fold_left_none in H1; simpl in *; intros; try destr. easy.
+          simpl in H1. rewrite fold_left_none in H1; simpl in *;
+          intros; try destr. easy.
           auto. auto.
       + rewrite fold_left_none; auto.
         split; intros A. 2: inv A.
@@ -388,483 +390,377 @@ Section Interp.
         apply iok in H6. rewrite H6 in Heqo; inv Heqo. auto.
   Qed.
 
-  
   Inductive interp_action:
-    forall {reg_t ext_fn_t: Type}
-           `{REnv: Env reg_t}
-           (r: REnv.(env_t) (fun _ => val))
-           (sigma: forall f: ext_fn_t, val -> val)
-           (Gamma: list (var_t * val))
-           (sched_log: Log REnv)
-           (action_log: Log REnv)
-           (a: Syntax.uaction pos_t var_t fn_name_t reg_t ext_fn_t)
-           (action_log': Log REnv)
-           (res: val)
-           (Gamma': list (var_t * val)), Prop :=
+    forall
+      {reg_t ext_fn_t: Type} `{REnv: Env reg_t} (r: REnv.(env_t) (fun _ => val))
+      (sigma: forall f: ext_fn_t, val -> val) (Gamma: list (var_t * val))
+      (sched_log: Log REnv) (action_log: Log REnv)
+      (a: Syntax.uaction pos_t var_t fn_name_t reg_t ext_fn_t)
+      (action_log': Log REnv) (res: val) (Gamma': list (var_t * val)),
+    Prop
+  :=
   | interp_action_var:
-    forall {reg_t ext_fn_t: Type}
-           `{REnv: Env reg_t}
-           (r: REnv.(env_t) (fun _ => val))
-           (sigma: forall f: ext_fn_t, val -> val)
-           (Gamma: list (var_t * val))
-           (sched_log: Log REnv)
-           (action_log: Log REnv)
-           var v,
-      list_assoc Gamma var = Some v ->
-      interp_action r sigma Gamma sched_log action_log (UVar var) action_log v Gamma
+    forall
+      {reg_t ext_fn_t: Type} `{REnv: Env reg_t} (r: REnv.(env_t) (fun _ => val))
+      (sigma: forall f: ext_fn_t, val -> val) (Gamma: list (var_t * val))
+      (sched_log: Log REnv) (action_log: Log REnv) var v,
+    list_assoc Gamma var = Some v
+    -> interp_action
+      r sigma Gamma sched_log action_log (UVar var) action_log v Gamma
   | interp_action_const:
-    forall {reg_t ext_fn_t: Type}
-           {REnv: Env reg_t}
-           (r: REnv.(env_t) (fun _ => val))
-           (sigma: forall f: ext_fn_t, val -> val)
-           (Gamma: list (var_t * val))
-           (sched_log: Log REnv)
-           (action_log: Log REnv)
-           tau (cst: type_denote tau),
-      interp_action r sigma Gamma sched_log action_log (UConst cst) action_log (val_of_value cst) Gamma
+    forall
+      {reg_t ext_fn_t: Type} {REnv: Env reg_t} (r: REnv.(env_t) (fun _ => val))
+      (sigma: forall f: ext_fn_t, val -> val) (Gamma: list (var_t * val))
+      (sched_log: Log REnv) (action_log: Log REnv) tau (cst: type_denote tau),
+    interp_action
+      r sigma Gamma sched_log action_log (UConst cst) action_log
+      (val_of_value cst) Gamma
   | interp_action_assign:
-    forall {reg_t ext_fn_t: Type}
-           {REnv: Env reg_t}
-           (r: REnv.(env_t) (fun _ => val))
-           (sigma: forall f: ext_fn_t, val -> val)
-           (Gamma: list (var_t * val))
-           (sched_log: Log REnv)
-           (action_log: Log REnv)
-           k a action_log' Gamma' v,
-      interp_action r sigma Gamma sched_log action_log a action_log' v Gamma' ->
-      interp_action r sigma Gamma sched_log action_log (UAssign k a) action_log' (Bits 0 [])
-                    (list_assoc_set Gamma' k v)
+    forall
+      {reg_t ext_fn_t: Type} {REnv: Env reg_t} (r: REnv.(env_t) (fun _ => val))
+      (sigma: forall f: ext_fn_t, val -> val) (Gamma: list (var_t * val))
+      (sched_log: Log REnv) (action_log: Log REnv) k a action_log' Gamma' v,
+    interp_action r sigma Gamma sched_log action_log a action_log' v Gamma'
+    -> interp_action
+      r sigma Gamma sched_log action_log (UAssign k a) action_log' (Bits 0 [])
+      (list_assoc_set Gamma' k v)
   | interp_action_seq:
-    forall {reg_t ext_fn_t: Type}
-           {REnv: Env reg_t}
-           (r: REnv.(env_t) (fun _ => val))
-           (sigma: forall f: ext_fn_t, val -> val)
-           (Gamma: list (var_t * val))
-           (sched_log: Log REnv)
-           (action_log: Log REnv)
-           a1 a2 v1 v2 action_log' Gamma' action_log'' Gamma'',
-      interp_action r sigma Gamma sched_log action_log a1 action_log' v1 Gamma' ->
-      interp_action r sigma Gamma' sched_log action_log' a2 action_log'' v2 Gamma'' ->
-      interp_action r sigma Gamma sched_log action_log (USeq a1 a2) action_log'' v2
-                    Gamma''
+    forall
+      {reg_t ext_fn_t: Type} {REnv: Env reg_t} (r: REnv.(env_t) (fun _ => val))
+      (sigma: forall f: ext_fn_t, val -> val) (Gamma: list (var_t * val))
+      (sched_log: Log REnv) (action_log: Log REnv) a1 a2 v1 v2 action_log'
+      Gamma' action_log'' Gamma'',
+    interp_action r sigma Gamma sched_log action_log a1 action_log' v1 Gamma'
+    -> interp_action
+      r sigma Gamma' sched_log action_log' a2 action_log'' v2 Gamma''
+    -> interp_action
+      r sigma Gamma sched_log action_log (USeq a1 a2) action_log'' v2 Gamma''
   | interp_action_bind:
-    forall {reg_t ext_fn_t: Type}
-           {REnv: Env reg_t}
-           (r: REnv.(env_t) (fun _ => val))
-           (sigma: forall f: ext_fn_t, val -> val)
-           (Gamma: list (var_t * val))
-           (sched_log: Log REnv)
-           (action_log: Log REnv)
-           k a1 a2 v1 v2 action_log' Gamma' action_log'' Gamma'',
-      interp_action r sigma Gamma sched_log action_log a1 action_log' v1 Gamma' ->
-      interp_action r sigma ((k,v1)::Gamma') sched_log action_log' a2 action_log'' v2 Gamma'' ->
-      interp_action r sigma Gamma sched_log action_log (UBind k a1 a2) action_log'' v2
-                    (tl Gamma'')
+    forall
+      {reg_t ext_fn_t: Type} {REnv: Env reg_t} (r: REnv.(env_t) (fun _ => val))
+      (sigma: forall f: ext_fn_t, val -> val) (Gamma: list (var_t * val))
+      (sched_log: Log REnv) (action_log: Log REnv) k a1 a2 v1 v2 action_log'
+      Gamma' action_log'' Gamma'',
+    interp_action r sigma Gamma sched_log action_log a1 action_log' v1 Gamma'
+    -> interp_action
+      r sigma ((k,v1)::Gamma') sched_log action_log' a2 action_log'' v2 Gamma''
+    -> interp_action r sigma Gamma sched_log action_log (UBind k a1 a2)
+      action_log'' v2 (tl Gamma'')
   | interp_action_if:
-    forall {reg_t ext_fn_t: Type}
-           {REnv: Env reg_t}
-           (r: REnv.(env_t) (fun _ => val))
-           (sigma: forall f: ext_fn_t, val -> val)
-           (Gamma: list (var_t * val))
-           (sched_log: Log REnv)
-           (action_log: Log REnv)
-           cond b athen aelse v2 action_log' Gamma' action_log'' Gamma'',
-      interp_action r sigma Gamma sched_log action_log cond action_log' (Bits 1 [b]) Gamma' ->
-      interp_action r sigma Gamma' sched_log action_log' (if b then athen else aelse)
-                    action_log'' v2 Gamma'' ->
-      interp_action r sigma Gamma sched_log action_log (UIf cond athen aelse) action_log'' v2
-                    Gamma''
+    forall
+      {reg_t ext_fn_t: Type} {REnv: Env reg_t} (r: REnv.(env_t) (fun _ => val))
+      (sigma: forall f: ext_fn_t, val -> val) (Gamma: list (var_t * val))
+      (sched_log: Log REnv) (action_log: Log REnv) cond b athen aelse v2
+      action_log' Gamma' action_log'' Gamma'',
+    interp_action
+      r sigma Gamma sched_log action_log cond action_log' (Bits 1 [b]) Gamma'
+    -> interp_action
+      r sigma Gamma' sched_log action_log' (if b then athen else aelse)
+      action_log'' v2 Gamma''
+    -> interp_action
+      r sigma Gamma sched_log action_log (UIf cond athen aelse) action_log'' v2
+      Gamma''
   | interp_action_read:
-    forall {reg_t ext_fn_t: Type}
-           {REnv: Env reg_t}
-           (r: REnv.(env_t) (fun _ => val))
-           (sigma: forall f: ext_fn_t, val -> val)
-           (Gamma: list (var_t * val))
-           (sched_log: Log REnv)
-           (action_log: Log REnv)
-           prt idx,
-      may_read sched_log prt idx = true ->
-      interp_action r sigma Gamma sched_log action_log
-                    (URead prt idx)
-                    (log_cons idx (LE Logs.LogRead prt (Bits 0 [])) action_log)
-                    (match prt with
-                    | P0 => REnv.(getenv) r idx
-                    | P1 => match latest_write0 (V:=val) (log_app action_log sched_log) idx with
-                            | Some v => v
-                            | None => REnv.(getenv) r idx
-                            end
-                    end)
-                    Gamma
-
+    forall
+      {reg_t ext_fn_t: Type} {REnv: Env reg_t} (r: REnv.(env_t) (fun _ => val))
+      (sigma: forall f: ext_fn_t, val -> val) (Gamma: list (var_t * val))
+      (sched_log: Log REnv) (action_log: Log REnv) prt idx,
+    may_read sched_log prt idx = true
+    -> interp_action
+      r sigma Gamma sched_log action_log (URead prt idx)
+      (log_cons idx (LE Logs.LogRead prt (Bits 0 [])) action_log)
+      ( match prt with
+        | P0 => REnv.(getenv) r idx
+        | P1 =>
+          match latest_write0 (V:=val) (log_app action_log sched_log) idx with
+          | Some v => v
+          | None => REnv.(getenv) r idx
+          end
+        end
+      )
+      Gamma
   | interp_action_write:
-    forall {reg_t ext_fn_t: Type}
-           {REnv: Env reg_t}
-           (r: REnv.(env_t) (fun _ => val))
-           (sigma: forall f: ext_fn_t, val -> val)
-           (Gamma: list (var_t * val))
-           (sched_log: Log REnv)
-           (action_log: Log REnv)
-           prt idx a v action_log' Gamma',
-      interp_action r sigma Gamma sched_log action_log a action_log' v Gamma' ->
-      may_write sched_log action_log' prt idx = true ->
-      interp_action r sigma Gamma sched_log action_log
-                    (UWrite prt idx a)
-                    (log_cons idx (LE Logs.LogWrite prt v) action_log')
-                    (Bits 0 [])
-                    Gamma'
-
+    forall
+      {reg_t ext_fn_t: Type} {REnv: Env reg_t} (r: REnv.(env_t) (fun _ => val))
+      (sigma: forall f: ext_fn_t, val -> val) (Gamma: list (var_t * val))
+      (sched_log: Log REnv) (action_log: Log REnv) prt idx a v action_log'
+      Gamma',
+    interp_action r sigma Gamma sched_log action_log a action_log' v Gamma'
+    -> may_write sched_log action_log' prt idx = true
+    -> interp_action
+      r sigma Gamma sched_log action_log (UWrite prt idx a)
+      (log_cons idx (LE Logs.LogWrite prt v) action_log') (Bits 0 []) Gamma'
   | interp_action_unop:
-    forall {reg_t ext_fn_t: Type}
-           {REnv: Env reg_t}
-           (r: REnv.(env_t) (fun _ => val))
-           (sigma: forall f: ext_fn_t, val -> val)
-           (Gamma: list (var_t * val))
-           (sched_log: Log REnv)
-           (action_log: Log REnv)
-           fn a v v' action_log' Gamma',
-      interp_action r sigma Gamma sched_log action_log a action_log' v Gamma' ->
-      sigma1 fn v = Some v' ->
-      interp_action r sigma Gamma sched_log action_log
-                    (UUnop fn a)
-                    action_log'
-                    v'
-                    Gamma'
-
+    forall
+      {reg_t ext_fn_t: Type} {REnv: Env reg_t} (r: REnv.(env_t) (fun _ => val))
+      (sigma: forall f: ext_fn_t, val -> val) (Gamma: list (var_t * val))
+      (sched_log: Log REnv) (action_log: Log REnv) fn a v v' action_log' Gamma',
+    interp_action r sigma Gamma sched_log action_log a action_log' v Gamma'
+    -> sigma1 fn v = Some v'
+    -> interp_action
+      r sigma Gamma sched_log action_log (UUnop fn a) action_log' v' Gamma'
   | interp_action_binop:
-    forall {reg_t ext_fn_t: Type}
-           {REnv: Env reg_t}
-           (r: REnv.(env_t) (fun _ => val))
-           (sigma: forall f: ext_fn_t, val -> val)
-           (Gamma: list (var_t * val))
-           (sched_log: Log REnv)
-           (action_log: Log REnv)
-           fn a1 a2 v1 v2 v'
-           action_log' Gamma'
-           action_log'' Gamma'',
-      interp_action r sigma Gamma sched_log action_log a1 action_log' v1 Gamma' ->
-      interp_action r sigma Gamma' sched_log action_log' a2 action_log'' v2 Gamma'' ->
-      sigma2 fn v1 v2 = Some v' ->
-      interp_action r sigma Gamma sched_log action_log
-                    (UBinop fn a1 a2)
-                    action_log''
-                    v'
-                    Gamma''
-
+    forall
+      {reg_t ext_fn_t: Type} {REnv: Env reg_t} (r: REnv.(env_t) (fun _ => val))
+      (sigma: forall f: ext_fn_t, val -> val) (Gamma: list (var_t * val))
+      (sched_log: Log REnv) (action_log: Log REnv) fn a1 a2 v1 v2 v' action_log'
+      Gamma' action_log'' Gamma'',
+    interp_action r sigma Gamma sched_log action_log a1 action_log' v1 Gamma'
+    -> interp_action
+      r sigma Gamma' sched_log action_log' a2 action_log'' v2 Gamma''
+    -> sigma2 fn v1 v2 = Some v'
+    -> interp_action
+      r sigma Gamma sched_log action_log (UBinop fn a1 a2) action_log'' v'
+      Gamma''
   | interp_action_extcall:
-    forall {reg_t ext_fn_t: Type}
-           {REnv: Env reg_t}
-           (r: REnv.(env_t) (fun _ => val))
-           (sigma: forall f: ext_fn_t, val -> val)
-           (Gamma: list (var_t * val))
-           (sched_log: Log REnv)
-           (action_log: Log REnv)
-           fn a v action_log' Gamma',
-      interp_action r sigma Gamma sched_log action_log a action_log' v Gamma' ->
-      interp_action r sigma Gamma sched_log action_log
-                    (UExternalCall fn a)
-                    action_log'
-                    (sigma fn v)
-                    Gamma'
-
+    forall
+      {reg_t ext_fn_t: Type} {REnv: Env reg_t} (r: REnv.(env_t) (fun _ => val))
+      (sigma: forall f: ext_fn_t, val -> val) (Gamma: list (var_t * val))
+      (sched_log: Log REnv) (action_log: Log REnv) fn a v action_log' Gamma',
+    interp_action r sigma Gamma sched_log action_log a action_log' v Gamma'
+    -> interp_action
+      r sigma Gamma sched_log action_log (UExternalCall fn a) action_log'
+      (sigma fn v) Gamma'
   | interp_action_intcall:
-    forall {reg_t ext_fn_t: Type}
-           {REnv: Env reg_t}
-           (r: REnv.(env_t) (fun _ => val))
-           (sigma: forall f: ext_fn_t, val -> val)
-           (Gamma: list (var_t * val))
-           (sched_log: Log REnv)
-           (action_log: Log REnv)
-           f args lv v action_log' Gamma' action_log'' Gamma'',
-      interp_list r sigma (interp_action r sigma)
-                  Gamma sched_log action_log args action_log' lv Gamma' ->
-      interp_action r sigma
-             (map (fun '(name, _, v) => (name, v))
-                  (combine (rev (int_argspec f)) lv)) sched_log action_log' (int_body f)
-             action_log'' v Gamma'' ->
-      interp_action r sigma Gamma sched_log action_log
-                    (UInternalCall f args)
-                    action_log''
-                    v
-                    Gamma'
-
-
+    forall
+      {reg_t ext_fn_t: Type} {REnv: Env reg_t} (r: REnv.(env_t) (fun _ => val))
+      (sigma: forall f: ext_fn_t, val -> val) (Gamma: list (var_t * val))
+      (sched_log: Log REnv) (action_log: Log REnv) f args lv v action_log'
+      Gamma' action_log'' Gamma'',
+    interp_list
+      r sigma (interp_action r sigma) Gamma sched_log action_log args
+      action_log' lv Gamma'
+    -> interp_action
+      r sigma (map (fun '(name, _, v) => (name, v))
+      (combine (rev (int_argspec f)) lv)) sched_log action_log' (int_body f)
+      action_log'' v Gamma''
+    -> interp_action
+      r sigma Gamma sched_log action_log (UInternalCall f args) action_log'' v
+      Gamma'
   | interp_action_pos:
-    forall {reg_t ext_fn_t: Type}
-           {REnv: Env reg_t}
-           (r: REnv.(env_t) (fun _ => val))
-           (sigma: forall f: ext_fn_t, val -> val)
-           (Gamma: list (var_t * val))
-           (sched_log: Log REnv)
-           (action_log: Log REnv)
-           p a v Gamma' action_log',
-      interp_action r sigma Gamma sched_log action_log a action_log' v Gamma' ->
-      interp_action r sigma Gamma sched_log action_log (UAPos p a) action_log' v Gamma'
-
+    forall
+      {reg_t ext_fn_t: Type} {REnv: Env reg_t} (r: REnv.(env_t) (fun _ => val))
+      (sigma: forall f: ext_fn_t, val -> val) (Gamma: list (var_t * val))
+      (sched_log: Log REnv) (action_log: Log REnv) p a v Gamma' action_log',
+    interp_action r sigma Gamma sched_log action_log a action_log' v Gamma'
+    -> interp_action
+      r sigma Gamma sched_log action_log (UAPos p a) action_log' v Gamma'
   | interp_action_skip:
-    forall {reg_t ext_fn_t: Type}
-           {REnv: Env reg_t}
-           (r: REnv.(env_t) (fun _ => val))
-           (sigma: forall f: ext_fn_t, val -> val)
-           (Gamma: list (var_t * val))
-           (sched_log: Log REnv)
-           (action_log: Log REnv)
-           ,
-      interp_action r sigma Gamma sched_log action_log (USugar USkip) action_log (Bits 0 []) Gamma
-
-
+    forall
+      {reg_t ext_fn_t: Type} {REnv: Env reg_t} (r: REnv.(env_t) (fun _ => val))
+      (sigma: forall f: ext_fn_t, val -> val) (Gamma: list (var_t * val))
+      (sched_log: Log REnv) (action_log: Log REnv) ,
+      interp_action
+        r sigma Gamma sched_log action_log (USugar USkip) action_log
+        (Bits 0 []) Gamma
   | interp_action_constbits:
-    forall {reg_t ext_fn_t: Type}
-           {REnv: Env reg_t}
-           (r: REnv.(env_t) (fun _ => val))
-           (sigma: forall f: ext_fn_t, val -> val)
-           (Gamma: list (var_t * val))
-           (sched_log: Log REnv)
-           (action_log: Log REnv)
-           n (v: bits n),
-      let l := vect_to_list v in
-      interp_action r sigma Gamma sched_log action_log (USugar (UConstBits v))
-                    action_log (Bits (List.length l) l) Gamma
-
+    forall
+      {reg_t ext_fn_t: Type} {REnv: Env reg_t} (r: REnv.(env_t) (fun _ => val))
+      (sigma: forall f: ext_fn_t, val -> val) (Gamma: list (var_t * val))
+      (sched_log: Log REnv) (action_log: Log REnv) n (v: bits n),
+    let l := vect_to_list v in
+    interp_action
+      r sigma Gamma sched_log action_log (USugar (UConstBits v)) action_log
+      (Bits (List.length l) l) Gamma
   | interp_action_conststring:
-    forall {reg_t ext_fn_t: Type}
-           {REnv: Env reg_t}
-           (r: REnv.(env_t) (fun _ => val))
-           (sigma: forall f: ext_fn_t, val -> val)
-           (Gamma: list (var_t * val))
-           (sched_log: Log REnv)
-           (action_log: Log REnv)
-           s,
-
-      interp_action r sigma Gamma sched_log action_log (USugar (UConstString s))
-                    action_log (Array {| array_type := bits_t 8; array_len := String.length s |}
-                                      (List.map (fun x => Bits 8 (vect_to_list x)) (vect_to_list (SyntaxMacros.array_of_bytes s)))) Gamma
-
+    forall
+      {reg_t ext_fn_t: Type} {REnv: Env reg_t} (r: REnv.(env_t) (fun _ => val))
+      (sigma: forall f: ext_fn_t, val -> val) (Gamma: list (var_t * val))
+      (sched_log: Log REnv) (action_log: Log REnv) s,
+    interp_action
+      r sigma Gamma sched_log action_log (USugar (UConstString s)) action_log
+      (Array
+        {| array_type := bits_t 8; array_len := String.length s |}
+        (List.map
+          (fun x => Bits 8 (vect_to_list x))
+          (vect_to_list (SyntaxMacros.array_of_bytes s))
+        )
+      )
+      Gamma
   | interp_action_constenum:
-    forall {reg_t ext_fn_t: Type}
-           {REnv: Env reg_t}
-           (r: REnv.(env_t) (fun _ => val))
-           (sigma: forall f: ext_fn_t, val -> val)
-           (Gamma: list (var_t * val))
-           (sched_log: Log REnv)
-           (action_log: Log REnv)
-           sig name idx,
-      vect_index name sig.(enum_members) = Some idx ->
-      interp_action r sigma Gamma sched_log action_log (USugar (UConstEnum sig name))
-                    action_log (val_of_value (tau:= enum_t sig) (vect_nth sig.(enum_bitpatterns) idx)) Gamma
-
+    forall
+      {reg_t ext_fn_t: Type} {REnv: Env reg_t} (r: REnv.(env_t) (fun _ => val))
+      (sigma: forall f: ext_fn_t, val -> val) (Gamma: list (var_t * val))
+      (sched_log: Log REnv) (action_log: Log REnv) sig name idx,
+    vect_index name sig.(enum_members) = Some idx
+    -> interp_action
+      r sigma Gamma sched_log action_log (USugar (UConstEnum sig name))
+      action_log
+      (val_of_value (tau:= enum_t sig) (vect_nth sig.(enum_bitpatterns) idx))
+      Gamma
   | interp_action_progn:
-    forall {reg_t ext_fn_t: Type}
-           {REnv: Env reg_t}
-           (r: REnv.(env_t) (fun _ => val))
-           (sigma: forall f: ext_fn_t, val -> val)
-           (Gamma: list (var_t * val))
-           (sched_log: Log REnv)
-           (action_log: Log REnv)
-           aa Gamma' action_log' lv,
-      interp_list r sigma (interp_action r sigma) Gamma sched_log action_log aa action_log' lv Gamma' ->
-      interp_action r sigma Gamma sched_log action_log (USugar (UProgn aa))
-                    action_log'
-                    (List.hd (Bits 0 []) lv)
-                    Gamma'
-
+    forall
+      {reg_t ext_fn_t: Type} {REnv: Env reg_t} (r: REnv.(env_t) (fun _ => val))
+      (sigma: forall f: ext_fn_t, val -> val) (Gamma: list (var_t * val))
+      (sched_log: Log REnv) (action_log: Log REnv) aa Gamma' action_log' lv,
+    interp_list
+      r sigma (interp_action r sigma) Gamma sched_log action_log aa action_log'
+      lv Gamma'
+    -> interp_action
+      r sigma Gamma sched_log action_log (USugar (UProgn aa)) action_log'
+      (List.hd (Bits 0 []) lv) Gamma'
   | interp_action_let:
-    forall {reg_t ext_fn_t: Type}
-           {REnv: Env reg_t}
-           (r: REnv.(env_t) (fun _ => val))
-           (sigma: forall f: ext_fn_t, val -> val)
-           (Gamma: list (var_t * val))
-           (sched_log: Log REnv)
-           (action_log: Log REnv)
-           bindings body action_log' action_log'' Gamma' Gamma'' v,
-      interp_list_ctx r sigma (interp_action r sigma)
-                      Gamma sched_log action_log bindings action_log' Gamma' ->
-      interp_action r sigma Gamma' sched_log action_log' body action_log'' v Gamma'' ->
-      interp_action r sigma Gamma sched_log action_log (USugar (ULet bindings body))
-                    action_log''
-                    v
-                    (Nat.iter (List.length bindings) (@tl _) Gamma'')
-
-
+    forall
+      {reg_t ext_fn_t: Type} {REnv: Env reg_t} (r: REnv.(env_t) (fun _ => val))
+      (sigma: forall f: ext_fn_t, val -> val) (Gamma: list (var_t * val))
+      (sched_log: Log REnv) (action_log: Log REnv) bindings body action_log'
+      action_log'' Gamma' Gamma'' v,
+    interp_list_ctx
+      r sigma (interp_action r sigma) Gamma sched_log action_log bindings
+      action_log' Gamma'
+    -> interp_action
+      r sigma Gamma' sched_log action_log' body action_log'' v Gamma''
+    -> interp_action
+      r sigma Gamma sched_log action_log (USugar (ULet bindings body))
+      action_log'' v (Nat.iter (List.length bindings) (@tl _) Gamma'')
   | interp_action_when:
-    forall {reg_t ext_fn_t: Type}
-           {REnv: Env reg_t}
-           (r: REnv.(env_t) (fun _ => val))
-           (sigma: forall f: ext_fn_t, val -> val)
-           (Gamma: list (var_t * val))
-           (sched_log: Log REnv)
-           (action_log: Log REnv)
-           cond athen v2 action_log' Gamma' action_log'' Gamma'',
-      interp_action r sigma Gamma sched_log action_log cond action_log' (Bits 1 [true]) Gamma' ->
-      interp_action r sigma Gamma' sched_log action_log' athen
-                    action_log'' v2 Gamma'' ->
-      interp_action r sigma Gamma sched_log action_log (USugar (UWhen cond athen)) action_log'' v2
-                    Gamma''
-
-
+    forall
+      {reg_t ext_fn_t: Type} {REnv: Env reg_t} (r: REnv.(env_t) (fun _ => val))
+      (sigma: forall f: ext_fn_t, val -> val) (Gamma: list (var_t * val))
+      (sched_log: Log REnv) (action_log: Log REnv) cond athen v2 action_log'
+      Gamma' action_log'' Gamma'',
+    interp_action
+      r sigma Gamma sched_log action_log cond action_log' (Bits 1 [true]) Gamma'
+    -> interp_action
+      r sigma Gamma' sched_log action_log' athen action_log'' v2 Gamma''
+    -> interp_action
+      r sigma Gamma sched_log action_log (USugar (UWhen cond athen))
+      action_log'' v2 Gamma''
   | interp_action_switch_nil:
-      forall {reg_t ext_fn_t: Type}
-             {REnv: Env reg_t}
-             (r: REnv.(env_t) (fun _ => val))
-             (sigma: forall f: ext_fn_t, val -> val)
-             (Gamma: list (var_t * val))
-             (sched_log: Log REnv)
-             (action_log: Log REnv)
-             var default v action_log' Gamma',
-        interp_action r sigma Gamma sched_log action_log default action_log' v Gamma' ->
-        interp_action r sigma Gamma sched_log action_log (USugar (USwitch var default [])) action_log' v Gamma'
-
+    forall
+      {reg_t ext_fn_t: Type} {REnv: Env reg_t} (r: REnv.(env_t) (fun _ => val))
+      (sigma: forall f: ext_fn_t, val -> val) (Gamma: list (var_t * val))
+      (sched_log: Log REnv) (action_log: Log REnv) var default v action_log'
+      Gamma',
+    interp_action
+      r sigma Gamma sched_log action_log default action_log' v Gamma'
+    -> interp_action
+      r sigma Gamma sched_log action_log (USugar (USwitch var default []))
+      action_log' v Gamma'
   | interp_action_switch_ok:
-    forall {reg_t ext_fn_t: Type}
-           {REnv: Env reg_t}
-           (r: REnv.(env_t) (fun _ => val))
-           (sigma: forall f: ext_fn_t, val -> val)
-           (Gamma: list (var_t * val))
-           (sched_log: Log REnv)
-           (action_log: Log REnv)
-           var default cond body branches
-           action_log' Gamma'
-           action_log'' Gamma''
-           action_log''' Gamma'''
-           v0 v v2,
-      interp_action r sigma Gamma sched_log action_log var action_log' v0 Gamma' ->
-      interp_action r sigma Gamma' sched_log action_log' cond action_log'' v Gamma'' ->
-      v = v0 ->
-      interp_action r sigma Gamma'' sched_log action_log'' body action_log''' v2 Gamma''' ->
-      interp_action r sigma Gamma sched_log action_log
-                    (USugar (USwitch var default ((cond,body)::branches))) action_log''' v2
-                    Gamma'''
-
+    forall
+      {reg_t ext_fn_t: Type} {REnv: Env reg_t} (r: REnv.(env_t) (fun _ => val))
+      (sigma: forall f: ext_fn_t, val -> val) (Gamma: list (var_t * val))
+      (sched_log: Log REnv) (action_log: Log REnv) var default cond body
+      branches action_log' Gamma' action_log'' Gamma'' action_log''' Gamma''' v0
+      v v2,
+    interp_action r sigma Gamma sched_log action_log var action_log' v0 Gamma'
+    -> interp_action
+      r sigma Gamma' sched_log action_log' cond action_log'' v Gamma''
+    -> v = v0
+    -> interp_action
+      r sigma Gamma'' sched_log action_log'' body action_log''' v2 Gamma'''
+    -> interp_action
+      r sigma Gamma sched_log action_log
+      (USugar (USwitch var default ((cond,body)::branches))) action_log''' v2
+      Gamma'''
   | interp_action_switch_ko:
-    forall {reg_t ext_fn_t: Type}
-           {REnv: Env reg_t}
-           (r: REnv.(env_t) (fun _ => val))
-           (sigma: forall f: ext_fn_t, val -> val)
-           (Gamma: list (var_t * val))
-           (sched_log: Log REnv)
-           (action_log: Log REnv)
-            var default cond body branches
-           action_log' Gamma'
-           action_log'' Gamma''
-           action_log''' Gamma'''
-           v0 v v2,
-      interp_action r sigma Gamma sched_log action_log var action_log' v0 Gamma' ->
-      interp_action r sigma Gamma' sched_log action_log' cond action_log'' v Gamma'' ->
-      v <> v0 ->
-      interp_action r sigma Gamma'' sched_log action_log''
-                    (USugar (USwitch var default branches)) action_log''' v2
-                    Gamma''' ->
-      interp_action r sigma Gamma sched_log action_log
-                    (USugar (USwitch var default ((cond,body)::branches))) action_log''' v2
-                    Gamma'''
-
+    forall
+      {reg_t ext_fn_t: Type} {REnv: Env reg_t} (r: REnv.(env_t) (fun _ => val))
+      (sigma: forall f: ext_fn_t, val -> val) (Gamma: list (var_t * val))
+      (sched_log: Log REnv) (action_log: Log REnv) var default cond body
+      branches action_log' Gamma' action_log'' Gamma'' action_log''' Gamma''' v0
+      v v2,
+    interp_action r sigma Gamma sched_log action_log var action_log' v0 Gamma'
+    -> interp_action
+      r sigma Gamma' sched_log action_log' cond action_log'' v Gamma''
+    -> v <> v0 ->
+      interp_action
+        r sigma Gamma'' sched_log action_log''
+        (USugar (USwitch var default branches)) action_log''' v2 Gamma'''
+    -> interp_action
+      r sigma Gamma sched_log action_log
+      (USugar (USwitch var default ((cond,body)::branches))) action_log''' v2
+      Gamma'''
   | interp_action_structinit:
-    forall {reg_t ext_fn_t: Type}
-           {REnv: Env reg_t}
-           (r: REnv.(env_t) (fun _ => val))
-           (sigma: forall f: ext_fn_t, val -> val)
-           (Gamma: list (var_t * val))
-           (sched_log: Log REnv)
-           (action_log: Log REnv)
-           sig fields vfields action_log' Gamma' vs v,
-      interp_list r sigma (interp_action r sigma)
-                  Gamma sched_log action_log (map snd fields) action_log' vfields Gamma' ->
-      let zeroes := repeat false (struct_fields_sz (struct_fields sig)) in
-      uvalue_of_struct_bits (struct_fields sig) zeroes = Some vs ->
-      List.fold_left (fun vs '(name, v) =>
-                        let/opt vs := vs in
-                        subst_field_name (struct_fields sig) name v vs
-                     ) (combine (map fst fields) (rev vfields)) (Some vs) = Some v ->
-      interp_action r sigma Gamma sched_log action_log
-                    (USugar (UStructInit sig fields))
-                    action_log'
-                    (Struct sig v)
-                    Gamma'
-
+    forall
+      {reg_t ext_fn_t: Type} {REnv: Env reg_t} (r: REnv.(env_t) (fun _ => val))
+      (sigma: forall f: ext_fn_t, val -> val) (Gamma: list (var_t * val))
+      (sched_log: Log REnv) (action_log: Log REnv) sig fields vfields
+      action_log' Gamma' vs v,
+    interp_list
+      r sigma (interp_action r sigma) Gamma sched_log action_log
+      (map snd fields) action_log' vfields Gamma'
+    -> let zeroes := repeat false (struct_fields_sz (struct_fields sig)) in
+    uvalue_of_struct_bits (struct_fields sig) zeroes = Some vs
+    -> List.fold_left
+      (fun vs '(name, v) =>
+        let/opt vs := vs in
+        subst_field_name (struct_fields sig) name v vs
+      )
+      (combine (map fst fields) (rev vfields)) (Some vs)
+    = Some v
+    -> interp_action
+      r sigma Gamma sched_log action_log (USugar (UStructInit sig fields))
+      action_log' (Struct sig v) Gamma'
   | interp_action_arrayinit:
-    forall {reg_t ext_fn_t: Type}
-           {REnv: Env reg_t}
-           (r: REnv.(env_t) (fun _ => val))
-           (sigma: forall f: ext_fn_t, val -> val)
-           (Gamma: list (var_t * val))
-           (sched_log: Log REnv)
-           (action_log: Log REnv)
-           tau elements velts action_log' Gamma' vs v,
-      interp_list r sigma (interp_action r sigma)
-                  Gamma sched_log action_log elements action_log' velts Gamma' ->
-        let zeroes := repeat (repeat false (type_sz tau)) (List.length elements) in
-        uvalue_of_list_bits (tau:=tau) zeroes = Some vs ->
-        let sig := {| array_type := tau; array_len := List.length elements |} in
-      List.fold_left (fun acc v =>
-                        let/opt2 pos, vs := acc in
-                             let/opt2 l1, l2 := take_drop pos vs in
-                             match l2 with
-                               [] => None
-                             | a::l2 => Some (S pos, l1 ++ v :: l2)
-                             end
-                     ) (rev velts) (Some (0, vs)) = Some v ->
-      interp_action r sigma Gamma sched_log action_log
-                    (USugar (UArrayInit tau elements))
-                    action_log'
-                    (Array sig (snd v))
-                    Gamma'
-
+    forall
+      {reg_t ext_fn_t: Type} {REnv: Env reg_t} (r: REnv.(env_t) (fun _ => val))
+      (sigma: forall f: ext_fn_t, val -> val) (Gamma: list (var_t * val))
+      (sched_log: Log REnv) (action_log: Log REnv) tau elements velts
+      action_log' Gamma' vs v,
+    interp_list
+      r sigma (interp_action r sigma) Gamma sched_log action_log elements
+      action_log' velts Gamma'
+    ->
+    let zeroes := repeat (repeat false (type_sz tau)) (List.length elements)
+    in uvalue_of_list_bits (tau:=tau) zeroes = Some vs
+    -> let sig := {| array_type := tau; array_len := List.length elements |}
+    in List.fold_left
+      (fun acc v =>
+        let/opt2 pos, vs := acc in
+        let/opt2 l1, l2 := take_drop pos vs in
+        match l2 with
+        | [] => None
+        | a::l2 => Some (S pos, l1 ++ v :: l2)
+        end
+      )
+      (rev velts) (Some (0, vs))
+    = Some v
+    -> interp_action
+      r sigma Gamma sched_log action_log (USugar (UArrayInit tau elements))
+      action_log' (Array sig (snd v)) Gamma'
   | interp_action_callmodule:
-    forall {reg_t ext_fn_t: Type}
-           {REnv: Env reg_t}
-           (r: REnv.(env_t) (fun _ => val))
-           (sigma: forall f: ext_fn_t, val -> val)
-           (Gamma: list (var_t * val))
-           (sched_log: Log REnv)
-           (action_log: Log REnv)
-           module_reg_t module_ext_fn_t
-           `{finite: FiniteType module_reg_t}
-           (fR: module_reg_t -> reg_t)
-           (fSigma : module_ext_fn_t -> ext_fn_t)
-           fn args lv v action_log' Gamma' action_log'' Gamma'',
-      interp_list r sigma (interp_action r sigma)
-                  Gamma sched_log action_log args action_log' lv Gamma' ->
-      let REnv' := @ContextEnv _ _ in
-      interp_action (create REnv' (fun idx => getenv REnv r (fR idx)))
-                    (fun f => sigma (fSigma f))
-                    (map (fun '(name, _, v) => (name, v)) (combine (rev (int_argspec fn)) lv))
-                    (fLog fR REnv REnv' sched_log) (fLog fR REnv REnv' action_log')
-                    (int_body fn)
-             action_log'' v Gamma'' ->
-      interp_action r sigma Gamma sched_log action_log
-                    (USugar (UCallModule fR fSigma fn args))
-                    (fLog' fR REnv REnv' action_log'' action_log')
-                    v
-                    Gamma'
-
-
-  .
+    forall
+      {reg_t ext_fn_t: Type} {REnv: Env reg_t} (r: REnv.(env_t) (fun _ => val))
+      (sigma: forall f: ext_fn_t, val -> val) (Gamma: list (var_t * val))
+      (sched_log: Log REnv) (action_log: Log REnv) module_reg_t module_ext_fn_t
+      `{finite: FiniteType module_reg_t} (fR: module_reg_t -> reg_t)
+      (fSigma : module_ext_fn_t -> ext_fn_t) fn args lv v action_log' Gamma'
+      action_log'' Gamma'',
+    interp_list
+      r sigma (interp_action r sigma) Gamma sched_log action_log args
+      action_log' lv Gamma'
+    -> let REnv' := @ContextEnv _ _
+    in interp_action
+      (create REnv' (fun idx => getenv REnv r (fR idx)))
+      (fun f => sigma (fSigma f))
+      (map (fun '(name, _, v) => (name, v)) (combine (rev (int_argspec fn)) lv))
+      (fLog fR REnv REnv' sched_log) (fLog fR REnv REnv' action_log')
+      (int_body fn) action_log'' v Gamma''
+    -> interp_action
+      r sigma Gamma sched_log action_log
+      (USugar (UCallModule fR fSigma fn args))
+      (fLog' fR REnv REnv' action_log'' action_log') v Gamma'.
 
   Lemma list_assoc_eq_dec_ext:
     forall {K V: Type} {eq1 eq2: EqDec K} (l: list (K * V)) (k: K),
-      @list_assoc _ _ eq1 l k = @list_assoc _ _ eq2 l k.
-  Proof.
-    induction l; simpl; intros; eauto.
-    destr. repeat destr.
-  Qed.
+    @list_assoc _ _ eq1 l k = @list_assoc _ _ eq2 l k.
+  Proof. induction l; simpl; intros; eauto. destr. repeat destr. Qed.
 
   Lemma list_assoc_set_eq_dec_ext:
     forall {K V: Type} {eq1 eq2: EqDec K} (l: list (K * V)) (k: K) v,
-      @list_assoc_set _ _ eq1 l k v = @list_assoc_set _ _ eq2 l k v.
-  Proof.
-    induction l; simpl; intros; eauto.
-    destr. repeat destr.
-  Qed.
-
+    @list_assoc_set _ _ eq1 l k v = @list_assoc_set _ _ eq2 l k v.
+  Proof. induction l; simpl; intros; eauto. destr. repeat destr. Qed.
 
   Lemma ind_ok:
-    forall {reg_t ext_fn_t: Type}
-           a
-           (REnv: Env reg_t)
-           (r: REnv.(env_t) (fun _ => val))
-           (sigma: forall f: ext_fn_t, val -> val)
-           Gamma sched_log action_log Gamma' action_log' v,
-        UntypedSemantics.interp_action r sigma Gamma sched_log action_log a = Some (action_log', v, Gamma') <->
-        interp_action r sigma Gamma sched_log action_log a action_log' v Gamma'.
+    forall
+      {reg_t ext_fn_t: Type} a (REnv: Env reg_t)
+      (r: REnv.(env_t) (fun _ => val)) (sigma: forall f: ext_fn_t, val -> val)
+      Gamma sched_log action_log Gamma' action_log' v,
+    UntypedSemantics.interp_action
+      r sigma Gamma sched_log action_log a = Some (action_log', v, Gamma')
+    <-> interp_action r sigma Gamma sched_log action_log a action_log' v Gamma'.
   Proof.
     intros reg_t ext_fn_t ua. pattern reg_t, ext_fn_t , ua.
     match goal with
@@ -874,18 +770,15 @@ Section Interp.
     revert reg_t ext_fn_t ua Heqn.
     pattern n.
     eapply Nat.strong_right_induction with (z:=0).
-    {
-      red. red. intros. subst. tauto.
-    } 2: lia.
+    { red. red. intros. subst. tauto. } 2: lia.
     intros n0 _ Plt reg_t' ext_fn_t' ua Heqn. subst.
     assert (Plt':
-              forall reg_t ext_fn_t (a: Syntax.uaction pos_t var_t fn_name_t reg_t ext_fn_t),
-                size_uaction a < size_uaction ua -> PP reg_t ext_fn_t a
-           ).
-    {
-      intros. eapply Plt. 3: reflexivity. lia. auto.
-    } clear Plt.
-    rename Plt' into IHua. clear n. unfold PP.
+      forall
+        reg_t ext_fn_t (a: Syntax.uaction pos_t var_t fn_name_t reg_t ext_fn_t),
+      size_uaction a < size_uaction ua -> PP reg_t ext_fn_t a
+    ).
+    { intros. eapply Plt. 3: reflexivity. lia. auto. }
+    clear Plt. rename Plt' into IHua. clear n. unfold PP.
     destruct ua; simpl in *; intros.
     - split; intros A; inv A.
     - split; intros A; inv A.
@@ -905,7 +798,7 @@ Section Interp.
       unfold opt_bind in A; repeat destr_in A; inv A.
       eapply interp_action_assign. apply IHua.  lia. auto.
       dependent induction A. subst.
-      apply IHua in A. rewrite A. simpl. 
+      apply IHua in A. rewrite A. simpl.
       erewrite list_assoc_set_eq_dec_ext. eauto. lia.
     - split; intros A.
       unfold opt_bind in A; repeat destr_in A; inv A.
@@ -981,8 +874,7 @@ Section Interp.
         econstructor; eauto.
         cut (size_uaction a <= list_sum (map size_uaction args)).
         lia.
-        {
-          clear - H. revert H; induction args; simpl; intros; eauto. easy.
+        { clear - H. revert H; induction args; simpl; intros; eauto. easy.
           destruct H. subst. lia.
           apply IHargs in H. lia.
         }
@@ -994,8 +886,7 @@ Section Interp.
         intros; eapply IHua.
         cut (size_uaction a <= list_sum (map size_uaction args)).
         lia.
-        {
-          clear - H0. revert H0; induction args; simpl; intros; eauto. easy.
+        { clear - H0. revert H0; induction args; simpl; intros; eauto. easy.
           destruct H0. subst. lia.
           apply IHargs in H. lia.
         }
@@ -1024,25 +915,37 @@ Section Interp.
         * destr_in A; inv A. econstructor; eauto.
         * dependent induction A. subst. rewrite H. eauto.
       + assert (
-            forall aa v0 action_log Gamma,
-              fold_left
-                (fun (acc : option (Log REnv * val * list (var_t * val)))
-                     (a : uaction pos_t var_t fn_name_t reg_t' ext_fn_t') =>
-                   let/opt3 action_log, _, Gamma := acc
-                   in UntypedSemantics.interp_action r sigma Gamma sched_log action_log a) aa
-                (Some (action_log, v0, Gamma)) =
-              let/opt3 action_log, l, Gamma := fold_left
-                                                 (fun (acc : option (Log REnv * list val * list (var_t * val)))
-                                                      (a : uaction pos_t var_t fn_name_t reg_t' ext_fn_t') =>
-                                                    let/opt3 action_log, l, Gamma := acc in
-                                                    let/opt3 action_log, v, Gamma := UntypedSemantics.interp_action r sigma Gamma sched_log action_log a in
-                                                    Some(action_log, v::l, Gamma)) aa
-                                                 (Some (action_log, [], Gamma)) in
-          Some(action_log, hd v0 l, Gamma)).
-        {
-          clear.
+          forall aa v0 action_log Gamma,
+          fold_left
+            (fun
+              (acc : option (Log REnv * val * list (var_t * val)))
+              (a : uaction pos_t var_t fn_name_t reg_t' ext_fn_t')
+             =>
+               let/opt3 action_log, _, Gamma := acc in
+               UntypedSemantics.interp_action
+                r sigma Gamma sched_log action_log a
+            ) aa (Some (action_log, v0, Gamma))
+          = let/opt3 action_log, l, Gamma :=
+            fold_left
+              (fun
+                (acc : option (Log REnv * list val * list (var_t * val)))
+                (a : uaction pos_t var_t fn_name_t reg_t' ext_fn_t')
+              =>
+                let/opt3 action_log, l, Gamma := acc in
+                let/opt3 action_log, v, Gamma :=
+                  UntypedSemantics.interp_action
+                    r sigma Gamma sched_log action_log a
+                in Some(action_log, v::l, Gamma)
+              )
+              aa (Some (action_log, [], Gamma))
+          in Some(action_log, hd v0 l, Gamma)
+        ).
+        { clear.
           induction aa; simpl; intros; eauto.
-          destruct (UntypedSemantics.interp_action r sigma Gamma sched_log action_log a) eqn:?.
+          destruct (
+            UntypedSemantics.interp_action
+              r sigma Gamma sched_log action_log a
+          ) eqn:?.
           - destruct p, p; simpl.
             rewrite IHaa.
             rewrite fold_left_rec with (X:=[v]). destr; simpl; auto.
@@ -1056,10 +959,10 @@ Section Interp.
         split; intros A.
         * unfold opt_bind in A; destr_in A; simpl in *; try congruence.
           repeat destr_in A; inv A.
-          econstructor. eapply interp_list_ok; eauto. 2: setoid_rewrite Heqo; auto.
+          econstructor. eapply interp_list_ok; eauto.
+          2: setoid_rewrite Heqo; auto.
           intros; eapply IHua; eauto.
-          {
-            clear - H. revert H; induction aa; simpl; intros; eauto. easy.
+          { clear - H. revert H; induction aa; simpl; intros; eauto. easy.
             destruct H. subst. lia.
             apply IHaa in H. lia.
           }
@@ -1067,8 +970,7 @@ Section Interp.
           eapply interp_list_ok in H.
           rewrite H. simpl. auto.
           intros; eapply IHua; eauto.
-          {
-            clear - H1. revert H1; induction aa; simpl; intros; eauto. easy.
+          { clear - H1. revert H1; induction aa; simpl; intros; eauto. easy.
             destruct H1. subst. lia.
             apply IHaa in H. simpl in H. lia.
           }
@@ -1078,8 +980,7 @@ Section Interp.
           2: intros; eapply IHua.
           eapply IHua in Heqo0. 2: simpl; lia.
           econstructor; eauto.
-          {
-            clear - H. revert H; induction bindings; simpl; intros; eauto. easy.
+          { clear - H. revert H; induction bindings; simpl; intros; eauto. easy.
             destruct H. subst. destr. simpl in *. lia.
             apply IHbindings in H. simpl in H. destr. lia.
           }
@@ -1089,8 +990,7 @@ Section Interp.
           eapply IHua in A. 2: simpl; lia.
           rewrite A. simpl; auto.
           intros; eapply IHua.
-          {
-            clear - H1. rename H1 into H.
+          { clear - H1. rename H1 into H.
             revert H; induction bindings; simpl; intros; eauto. easy.
             destruct H. subst. destr. simpl in *. lia.
             apply IHbindings in H. simpl in H. destr. lia.
@@ -1109,26 +1009,37 @@ Section Interp.
           induction branches; simpl in *.
           -- inv Heqo.
           -- destruct a.
-             destruct (match UntypedSemantics.interp_action r sigma Gamma sched_log action_log var with
-           | Some (action_log, v0, Gamma) =>
-               match UntypedSemantics.interp_action r sigma Gamma sched_log action_log u with
-               | Some (action_log0, v, Gamma0) =>
-                   if val_eq_dec v v0
-                   then
-                    match UntypedSemantics.interp_action r sigma Gamma0 sched_log action_log0 u0 with
-                    | Some (action_log1, v1, Gamma1) => Some (action_log1, Some v1, Gamma1)
-                    | None => None
-                    end
+             destruct (
+               match
+                 UntypedSemantics.interp_action
+                   r sigma Gamma sched_log action_log var
+               with
+               | Some (action_log, v0, Gamma) =>
+                 match
+                   UntypedSemantics.interp_action
+                     r sigma Gamma sched_log action_log u
+                 with
+                 | Some (action_log0, v, Gamma0) =>
+                   if val_eq_dec v v0 then
+                     match
+                       UntypedSemantics.interp_action
+                         r sigma Gamma0 sched_log action_log0 u0
+                     with
+                     | Some (action_log1, v1, Gamma1) =>
+                       Some (action_log1, Some v1, Gamma1)
+                     | None => None
+                     end
                    else Some (action_log0, None, Gamma0)
+                 | None => None
+                 end
                | None => None
                end
-           | None => None
-           end) eqn:?.
-             2: rewrite fold_left_none in Heqo. 2: inv Heqo. 2: intros; destr; auto.
+             ) eqn:?.
+             2: rewrite fold_left_none in Heqo. 2: inv Heqo.
+             2: intros; destr; auto.
              repeat destr_in Heqo0; inv Heqo0.
              replace (fold_left _ _ _) with (Some (l4, Some v2, l3)) in Heqo.
-             2: {
-               clear.
+             2: { clear.
                induction branches; simpl; intros; eauto.
                destruct a; auto.
              }
@@ -1142,67 +1053,70 @@ Section Interp.
              eapply interp_action_switch_ko; eauto.
              eapply IHua. simpl. lia.
              simpl. setoid_rewrite Heqo. simpl. auto.
-          --
-            revert l l0 action_log Gamma Heqo H0.
-            induction branches; simpl; intros; eauto.
-            ++ eapply IHua in H0. 2: simpl; lia.
-               inv Heqo.
-               econstructor. eauto.
-            ++ destruct a.
-               destruct (match UntypedSemantics.interp_action r sigma Gamma sched_log action_log var with
-                         | Some (action_log, v0, Gamma) =>
-                           match UntypedSemantics.interp_action r sigma Gamma sched_log action_log u with
-                           | Some (action_log0, v, Gamma0) =>
-                             if val_eq_dec v v0
-                             then
-                               match UntypedSemantics.interp_action r sigma Gamma0 sched_log action_log0 u0 with
-                               | Some (action_log1, v1, Gamma1) => Some (action_log1, Some v1, Gamma1)
-                               | None => None
-                               end
-                             else Some (action_log0, None, Gamma0)
-                           | None => None
-                           end
-                         | None => None
-                         end) eqn:?.
-               2: rewrite fold_left_none in Heqo. 2: inv Heqo. 2: intros; destr; auto.
-               repeat destr_in Heqo0; inv Heqo0.
-               replace (fold_left _ _ _) with (Some (l6, Some v2, l5)) in Heqo.
-               2: {
-                 clear.
-                 induction branches; simpl; intros; eauto.
-                 destruct a; auto.
-               }
-               inv Heqo.
-               eapply IHua in Heqo1. 2: simpl; lia.
-               eapply IHua in Heqo2. 2: simpl; lia.
-               eapply IHua in H0. 2: simpl; lia.
-               eapply interp_action_switch_ko; eauto.
-               eapply IHbranches; eauto. simpl; intros; eapply IHua. simpl. lia.
-               eapply IHua. simpl. lia. eauto.
+          -- revert l l0 action_log Gamma Heqo H0.
+             induction branches; simpl; intros; eauto.
+             ++ eapply IHua in H0. 2: simpl; lia.
+                inv Heqo.
+                econstructor. eauto.
+             ++ destruct a.
+                destruct (
+                  match
+                    UntypedSemantics.interp_action
+                      r sigma Gamma sched_log action_log var
+                  with
+                  | Some (action_log, v0, Gamma) =>
+                    match
+                      UntypedSemantics.interp_action
+                        r sigma Gamma sched_log action_log u
+                    with
+                    | Some (action_log0, v, Gamma0) =>
+                      if val_eq_dec v v0 then
+                        match
+                          UntypedSemantics.interp_action
+                            r sigma Gamma0 sched_log action_log0 u0
+                        with
+                        | Some (action_log1, v1, Gamma1) =>
+                          Some (action_log1, Some v1, Gamma1)
+                        | None => None
+                      end
+                      else Some (action_log0, None, Gamma0)
+                    | None => None
+                    end
+                  | None => None
+                  end
+                ) eqn:?.
+                2: rewrite fold_left_none in Heqo. 2: inv Heqo.
+                2: intros; destr; auto.
+                repeat destr_in Heqo0; inv Heqo0.
+                replace (fold_left _ _ _) with (Some (l6, Some v2, l5)) in Heqo.
+                2: { clear.
+                  induction branches; simpl; intros; eauto.
+                  destruct a; auto.
+                }
+                inv Heqo.
+                eapply IHua in Heqo1. 2: simpl; lia.
+                eapply IHua in Heqo2. 2: simpl; lia.
+                eapply IHua in H0. 2: simpl; lia.
+                eapply interp_action_switch_ko; eauto.
+                eapply IHbranches; eauto. simpl; intros; eapply IHua. simpl.
+                lia. eapply IHua. simpl. lia. eauto.
         * dependent induction A; subst.
           -- eapply IHua in A. 2: simpl; lia.
              simpl. eauto.
-          -- eapply IHua in A1. 2: simpl; lia.
-             eapply IHua in A2. 2: simpl; lia.
-             eapply IHua in A3. 2: simpl; lia.
-             simpl.
-             rewrite A1. simpl.
-             rewrite A2. simpl.
-             rewrite A3. simpl.
+          -- eapply IHua in A1. 2: simpl; lia. eapply IHua in A2. 2: simpl; lia.
+             eapply IHua in A3. 2: simpl; lia. simpl.
+             rewrite A1. simpl. rewrite A2. simpl. rewrite A3. simpl.
              destruct (val_eq_dec v0 v0); try congruence.
-             replace (fold_left _ _ _) with (Some (action_log''', Some v2, Gamma''')).
-             2: {
-               clear.
+             replace (fold_left _ _ _)
+               with (Some (action_log''', Some v2, Gamma''')).
+             2: { clear.
                induction branches0; simpl; intros; eauto.
                destruct a; auto.
              }
              simpl. auto.
-          -- eapply IHua in A1. 2: simpl; lia.
-             eapply IHua in A2. 2: simpl; lia.
-             eapply IHua in A3. 2: simpl; lia.
-             simpl.
-             rewrite A1. simpl.
-             rewrite A2. simpl.
+          -- eapply IHua in A1. 2: simpl; lia. eapply IHua in A2. 2: simpl; lia.
+             eapply IHua in A3. 2: simpl; lia. simpl.
+             rewrite A1. simpl. rewrite A2. simpl.
              destruct (val_eq_dec v v0); try congruence.
              eapply IHA3; eauto.
              intros; eapply IHua. simpl in *. lia.
@@ -1212,8 +1126,7 @@ Section Interp.
           destruct Heqo0 as (vf & IL & FL).
           econstructor; eauto.
           intros; eapply IHua. simpl.
-          {
-            clear - H. revert H.
+          { clear - H. revert H.
             induction fields; simpl; intros; eauto. easy.
             destruct a0; simpl in *.
             destruct H. subst. lia.
@@ -1221,10 +1134,10 @@ Section Interp.
           }
         * dependent induction A. subst.
           unfold zeroes in *. rewrite H0. simpl.
-          edestruct (structinit_ind_ok r sigma (interp_action r sigma)) as [SIO _].
+          edestruct (structinit_ind_ok r sigma (interp_action r sigma))
+            as [SIO _].
           intros; eapply IHua. 2: rewrite SIO.
-          {
-            clear - H2. revert H2.
+          { clear - H2. revert H2.
             induction fields; simpl; intros; eauto. easy.
             destruct a0; simpl in *.
             destruct H2. subst. lia.
@@ -1239,18 +1152,17 @@ Section Interp.
           replace (l1) with (snd (n, l1)).
           econstructor; eauto. reflexivity.
           intros; eapply IHua. simpl.
-          {
-            clear - H. revert H.
+          { clear - H. revert H.
             induction elements; simpl; intros; eauto. easy.
             destruct H. subst. lia.
             apply IHelements in H. lia.
           }
         * dependent induction A. subst.
           unfold zeroes in *. rewrite H0. simpl.
-          edestruct (arrayinit_ind_ok r sigma (interp_action r sigma)) as [SIO _].
+          edestruct (arrayinit_ind_ok r sigma (interp_action r sigma))
+            as [SIO _].
           intros; eapply IHua. 2: rewrite SIO.
-          {
-            clear - H2. revert H2.
+          { clear - H2. revert H2.
             induction elements; simpl; intros; eauto. easy.
             destruct H2. subst. lia.
             apply IHelements in H. simpl in H. lia.
@@ -1265,8 +1177,7 @@ Section Interp.
           econstructor. eauto. apply IHua. simpl; lia. eauto.
           cut (size_uaction a <= list_sum (map size_uaction args)).
           simpl; lia.
-          {
-            clear - H. revert H; induction args; simpl; intros; eauto. easy.
+          { clear - H. revert H; induction args; simpl; intros; eauto. easy.
             destruct H. subst. lia.
             apply IHargs in H. lia.
           }
@@ -1279,41 +1190,34 @@ Section Interp.
           intros; eapply IHua.
           cut (size_uaction a <= list_sum (map size_uaction args)).
           simpl; lia.
-          {
-            clear - H0. revert H0; induction args; simpl; intros; eauto. easy.
+          { clear - H0. revert H0; induction args; simpl; intros; eauto. easy.
             destruct H0. subst. lia.
             apply IHargs in H. lia.
           }
   Qed.
 
   Inductive interp_rule:
-    forall {reg_t ext_fn_t: Type}
-           `{REnv: Env reg_t}
-           (r: REnv.(env_t) (fun _ => val))
-           (sigma: forall f: ext_fn_t, val -> val)
-           (sched_log: Log REnv)
-           (a: Syntax.uaction pos_t var_t fn_name_t reg_t ext_fn_t)
-           (action_log': Log REnv), Prop :=
+    forall
+      {reg_t ext_fn_t: Type} `{REnv: Env reg_t} (r: REnv.(env_t) (fun _ => val))
+      (sigma: forall f: ext_fn_t, val -> val) (sched_log: Log REnv)
+      (a: Syntax.uaction pos_t var_t fn_name_t reg_t ext_fn_t)
+      (action_log': Log REnv),
+    Prop :=
   | interp_rule_intro:
-    forall {reg_t ext_fn_t: Type}
-           `{REnv: Env reg_t}
-           (r: REnv.(env_t) (fun _ => val))
-           (sigma: forall f: ext_fn_t, val -> val)
-           (Gamma': list (var_t * val))
-           (sched_log: Log REnv)
-           (action_log': Log REnv) a v,
-      interp_action r sigma nil sched_log log_empty a action_log' v Gamma' ->
-      interp_rule r sigma sched_log a action_log'.
+    forall
+      {reg_t ext_fn_t: Type} `{REnv: Env reg_t} (r: REnv.(env_t) (fun _ => val))
+      (sigma: forall f: ext_fn_t, val -> val) (Gamma': list (var_t * val))
+      (sched_log: Log REnv) (action_log': Log REnv) a v,
+    interp_action r sigma nil sched_log log_empty a action_log' v Gamma'
+    -> interp_rule r sigma sched_log a action_log'.
 
   Lemma interp_rule_ind_ok:
-    forall {reg_t ext_fn_t: Type}
-           a
-           (REnv: Env reg_t)
-           (r: REnv.(env_t) (fun _ => val))
-           (sigma: forall f: ext_fn_t, val -> val)
-           sched_log action_log',
-        UntypedSemantics.interp_rule r sigma sched_log a = Some (action_log') <->
-        interp_rule r sigma sched_log a action_log'.
+    forall
+      {reg_t ext_fn_t: Type} a (REnv: Env reg_t)
+      (r: REnv.(env_t) (fun _ => val)) (sigma: forall f: ext_fn_t, val -> val)
+      sched_log action_log',
+    UntypedSemantics.interp_rule r sigma sched_log a = Some (action_log')
+    <-> interp_rule r sigma sched_log a action_log'.
   Proof.
     intros. unfold UntypedSemantics.interp_rule.
     split; intros A.
@@ -1326,60 +1230,51 @@ Section Interp.
 
   Section Scheduler.
     Context {reg_t ext_fn_t: Type}.
-    Context (rules: rule_name_t -> uaction pos_t var_t fn_name_t reg_t ext_fn_t).
+    Context
+      (rules: rule_name_t -> uaction pos_t var_t fn_name_t reg_t ext_fn_t).
 
     Inductive interp_try
-             {REnv: Env reg_t}
-             (r: REnv.(env_t) (fun _ => val))
-             (sigma: forall f: ext_fn_t, val -> val)
-             (IS: Log REnv -> scheduler pos_t rule_name_t -> Log REnv -> Prop)
-      : Log REnv ->
-        rule_name_t ->
-        scheduler pos_t rule_name_t ->
-        scheduler pos_t rule_name_t ->
-        Log REnv ->
-        Prop :=
+      {REnv: Env reg_t} (r: REnv.(env_t) (fun _ => val))
+      (sigma: forall f: ext_fn_t, val -> val)
+      (IS: Log REnv -> scheduler pos_t rule_name_t -> Log REnv -> Prop)
+    : Log REnv -> rule_name_t -> scheduler pos_t rule_name_t
+      -> scheduler pos_t rule_name_t -> Log REnv -> Prop
+    :=
     | interp_try_ok:
-        forall sched_log rl l s1 s2 l',
-          interp_rule r sigma sched_log (rules rl) l ->
-          IS (log_app l sched_log) s1 l' ->
-          interp_try r sigma IS sched_log rl s1 s2 l'
+      forall sched_log rl l s1 s2 l',
+      interp_rule r sigma sched_log (rules rl) l ->
+      IS (log_app l sched_log) s1 l' ->
+      interp_try r sigma IS sched_log rl s1 s2 l'
     | interp_try_ko:
-        forall sched_log rl s1 s2 l',
-          (forall l, ~ interp_rule r sigma sched_log (rules rl) l) ->
-          IS sched_log s2 l' ->
-          interp_try r sigma IS sched_log rl s1 s2 l'
-    .
+      forall sched_log rl s1 s2 l',
+      (forall l, ~ interp_rule r sigma sched_log (rules rl) l) ->
+      IS sched_log s2 l' ->
+      interp_try r sigma IS sched_log rl s1 s2 l'.
 
     Inductive interp_scheduler'
-             {REnv: Env reg_t}
-             (r: REnv.(env_t) (fun _ => val))
-             (sigma: forall f: ext_fn_t, val -> val):
-      Log REnv -> scheduler pos_t rule_name_t -> Log REnv -> Prop :=
-    | interp_scheduler'_done:
-        forall l,
-          interp_scheduler' r sigma l Done l
+      {REnv: Env reg_t} (r: REnv.(env_t) (fun _ => val))
+      (sigma: forall f: ext_fn_t, val -> val)
+    : Log REnv -> scheduler pos_t rule_name_t -> Log REnv -> Prop :=
+    | interp_scheduler'_done: forall l, interp_scheduler' r sigma l Done l
     | interp_scheduler'_cons:
-        forall l rl s l',
-          interp_try r sigma (interp_scheduler' r sigma) l rl s s l' ->
-          interp_scheduler' r sigma l (Cons rl s) l'
+      forall l rl s l',
+      interp_try r sigma (interp_scheduler' r sigma) l rl s s l'
+      -> interp_scheduler' r sigma l (Cons rl s) l'
     | interp_scheduler'_try:
-        forall l rl s1 s2 l',
-          interp_try r sigma (interp_scheduler' r sigma) l rl s1 s2 l' ->
-          interp_scheduler' r sigma l (Try rl s1 s2) l'
+      forall l rl s1 s2 l',
+      interp_try r sigma (interp_scheduler' r sigma) l rl s1 s2 l'
+      -> interp_scheduler' r sigma l (Try rl s1 s2) l'
     | interp_scheduler'_spos:
-        forall l p s l',
-          interp_scheduler' r sigma l s l' ->
-          interp_scheduler' r sigma l (SPos p s) l'.
+      forall l p s l',
+      interp_scheduler' r sigma l s l'
+      -> interp_scheduler' r sigma l (SPos p s) l'.
 
     Lemma interp_scheduler'_ind_ok:
-      forall {REnv: Env reg_t}
-             (r: REnv.(env_t) (fun _ => val))
-             (sigma: forall f: ext_fn_t, val -> val)
-             s
-             l l',
-        UntypedSemantics.interp_scheduler' rules r sigma l s = l' <->
-        interp_scheduler' r sigma l s l'.
+      forall
+        {REnv: Env reg_t} (r: REnv.(env_t) (fun _ => val))
+        (sigma: forall f: ext_fn_t, val -> val) s l l',
+      UntypedSemantics.interp_scheduler' rules r sigma l s = l'
+      <-> interp_scheduler' r sigma l s l'.
     Proof.
       induction s; simpl; intros; eauto.
       - split. intros A. inv A. constructor.
@@ -1392,7 +1287,7 @@ Section Interp.
           * apply IHs in A.
             econstructor.
             eapply interp_try_ko; eauto.
-            intros l0 IR. apply interp_rule_ind_ok in IR. congruence. 
+            intros l0 IR. apply interp_rule_ind_ok in IR. congruence.
         + intros A. inv A. inv H3.
           * apply IHs in H0.
             apply interp_rule_ind_ok in H. rewrite H. eauto.
@@ -1406,7 +1301,7 @@ Section Interp.
           * apply IHs2 in A.
             econstructor.
             eapply interp_try_ko; eauto.
-            intros l0 IR. apply interp_rule_ind_ok in IR. congruence. 
+            intros l0 IR. apply interp_rule_ind_ok in IR. congruence.
         + intros A. inv A. inv H4.
           * apply IHs1 in H0.
             apply interp_rule_ind_ok in H. rewrite H. eauto.
@@ -1415,25 +1310,20 @@ Section Interp.
       - rewrite IHs. split; intros A. econstructor; eauto. inv A; auto.
     Qed.
 
-
     Inductive interp_scheduler
-             {REnv: Env reg_t}
-             (r: REnv.(env_t) (fun _ => val))
-             (sigma: forall f: ext_fn_t, val -> val):
-      scheduler pos_t rule_name_t -> Log REnv -> Prop :=
+      {REnv: Env reg_t} (r: REnv.(env_t) (fun _ => val))
+      (sigma: forall f: ext_fn_t, val -> val)
+    : scheduler pos_t rule_name_t -> Log REnv -> Prop :=
     | interp_scheduler_intro:
-        forall s l,
-          interp_scheduler' r sigma log_empty s l ->
-          interp_scheduler r sigma s l.
+      forall s l,
+      interp_scheduler' r sigma log_empty s l -> interp_scheduler r sigma s l.
 
     Lemma interp_scheduler_ind_ok:
-      forall {REnv: Env reg_t}
-             (r: REnv.(env_t) (fun _ => val))
-             (sigma: forall f: ext_fn_t, val -> val)
-             s
-             l',
-        UntypedSemantics.interp_scheduler rules r sigma s = l' <->
-        interp_scheduler r sigma s l'.
+      forall
+        {REnv: Env reg_t} (r: REnv.(env_t) (fun _ => val))
+        (sigma: forall f: ext_fn_t, val -> val) s l',
+      UntypedSemantics.interp_scheduler rules r sigma s = l'
+      <-> interp_scheduler r sigma s l'.
     Proof.
       intros. unfold UntypedSemantics.interp_scheduler.
       rewrite interp_scheduler'_ind_ok. split; intros A.
@@ -1442,23 +1332,19 @@ Section Interp.
     Qed.
 
     Inductive interp_cycle
-             {REnv: Env reg_t}
-             (r: REnv.(env_t) (fun _ => val))
-             (sigma: forall f: ext_fn_t, val -> val):
-      scheduler pos_t rule_name_t -> REnv.(env_t) (fun _ => val) -> Prop :=
+      {REnv: Env reg_t} (r: REnv.(env_t) (fun _ => val))
+      (sigma: forall f: ext_fn_t, val -> val)
+    : scheduler pos_t rule_name_t -> REnv.(env_t) (fun _ => val) -> Prop :=
     | interp_cycle_intro:
-        forall s l,
-          interp_scheduler r sigma s l ->
-          interp_cycle r sigma s (commit_update r l).
+      forall s l, interp_scheduler r sigma s l
+      -> interp_cycle r sigma s (commit_update r l).
 
     Lemma interp_cycle_ind_ok:
-      forall {REnv: Env reg_t}
-             (r: REnv.(env_t) (fun _ => val))
-             (sigma: forall f: ext_fn_t, val -> val)
-             s
-             r',
-        UntypedSemantics.interp_cycle rules r sigma s = r' <->
-        interp_cycle r sigma s r'.
+      forall
+        {REnv: Env reg_t} (r: REnv.(env_t) (fun _ => val))
+        (sigma: forall f: ext_fn_t, val -> val) s r',
+      UntypedSemantics.interp_cycle rules r sigma s = r'
+      <-> interp_cycle r sigma s r'.
     Proof.
       intros. unfold UntypedSemantics.interp_cycle.
       split; intros A.
@@ -1467,7 +1353,5 @@ Section Interp.
       inv A.
       apply interp_scheduler_ind_ok in H. congruence.
     Qed.
-    
   End Scheduler.
-
 End Interp.
